\documentclass{article}
\usepackage[left=2cm, right=2cm, top=2cm]{geometry}
\usepackage[utf8]{inputenc}

\title{Home Assignment 1}
\author{Andr√© Hedesand}
\date{October 2018}

\begin{document}

\maketitle

\section{Solutions}

\begin{enumerate}
    \item
    \begin{enumerate}
        \item % 1a
            \emph{"Recursive systems are never stable"}
            \\
            \textbf{False.} 
            Recursive systems are IIR systems e.g. 
            $$ y(n) = \frac{1}{2}y(n-1) + x(n) $$
            If we by stability mean BIBO-stability we can simply prove that the system above is stable. The Z-transorm of the system above is
            $$ 
            Y(z) = \frac{1}{2}z^{-1}Y(z) + X(z) \Rightarrow
            Y(z)(1 - \frac{1}{2}z^{-1}) = X(z) \Rightarrow
            $$
            $$
            Y(z) = \frac{1}{1 - \frac{1}{2}z^{-1}}X(z) = 
            H(z) X(z) \Rightarrow 
            H(z) = \frac{1}{1 - \frac{1}{2}z^{-1}} \Rightarrow
            $$
            $$
            h(n) = (\frac{1}{2})^{n} u(n)
            $$
            
            By definition the system above is stable if
            $ \sum_{n=0}^{\infty} |(\frac{1}{2})^{n}| < \infty $.
            This is true because $(\frac{1}{2})^{n}$ goes to zero as $n$ goes to $\infty$.
        
        \item % 1b
            \emph{"A convolution of two sequences in the time domain corresponds to a multiplication of the Z transforms of the signals."}
            \\
            \textbf{True.} This is true by definition.
        
        \item % 1c
            \emph{"An FIR filter is always stable."}
            \\
            \textbf{True.}
            A FIR filter can be discribed with a difference equation:
            $$ y(n) = \sum_{k=0}^{N} a_k x(n-k)$$
            The system is stable as all $a_n < \infty$.
            
        \item % 1d
            \emph{A first order IIR filter is stable iff the absolute value of the value of the factor in front of $y(n-1)$ is greater than 1.}
            \\
            \textbf{False.} The opposite is true. We can prove this by contradiction: If we assume the statement above is true we get:
            
            $$
            y(n) = Ay(n-1) + x(n), A > 1
            $$
            \begin{center}
                \textit{and}
            \end{center}
            $$
            \sum_k |h(k)| < \infty
            $$
            
            Lets do the same Z-transform as in \emph{1a)}:
            $$
            y(n) = Ay(n-1) + x(n) \Rightarrow h(n) = A^nu(n)
            $$
            At last we get
            $$
            \sum_k |h(k)| < \infty \Rightarrow \sum_{n=0}^{\infty}|A^n| < \infty
            $$
            
            
    \end{enumerate} 
\end{enumerate}

\end{document}
